thys/Network_Security_Policy_Verification/Security_Invariants/SINVAR_SecGwExt_impl.thy
@@ -4,13 +4,13 @@ begin
 
 code_identifier code_module SINVAR_SecGwExt_impl => (Scala) SINVAR_SecGwExt
 
-subsubsection {* SecurityInvariant SecurityGatewayExtended List Implementation *}
+subsubsection {* SecurityInvariant PolEnforcePointExtended List Implementation *}
 
 fun sinvar :: "'v list_graph \<Rightarrow> ('v \<Rightarrow> SINVAR_SecGwExt.secgw_member) \<Rightarrow> bool" where
   "sinvar G nP = (\<forall> (e1,e2) \<in> set (edgesL G). e1 \<noteq> e2 \<longrightarrow> SINVAR_SecGwExt.allowed_secgw_flow (nP e1) (nP e2))"
 
-definition SecurityGatewayExtended_offending_list:: "'v list_graph \<Rightarrow> ('v \<Rightarrow> secgw_member) \<Rightarrow> ('v \<times> 'v) list list" where
-  "SecurityGatewayExtended_offending_list G nP = (if sinvar G nP then
+definition PolEnforcePointExtended_offending_list:: "'v list_graph \<Rightarrow> ('v \<Rightarrow> secgw_member) \<Rightarrow> ('v \<times> 'v) list list" where
+  "PolEnforcePointExtended_offending_list G nP = (if sinvar G nP then
     []
    else 
     [ [e \<leftarrow> edgesL G. case e of (e1,e2) \<Rightarrow> e1 \<noteq> e2 \<and> \<not> allowed_secgw_flow (nP e1) (nP e2)] ])"
@@ -22,46 +22,46 @@ lemma[code_unfold]: "SecurityInvariant.node_props SINVAR_SecGwExt.default_node_p
 apply(simp add: NetModel_node_props_def)
 done
 
-definition "SecurityGateway_eval G P = (wf_list_graph G \<and>
+definition "PolEnforcePoint_eval G P = (wf_list_graph G \<and>
   sinvar G (SecurityInvariant.node_props SINVAR_SecGwExt.default_node_properties P))"
 
 
-interpretation SecurityGateway_impl:TopoS_List_Impl 
+interpretation PolEnforcePoint_impl:TopoS_List_Impl 
   where default_node_properties=SINVAR_SecGwExt.default_node_properties
   and sinvar_spec=SINVAR_SecGwExt.sinvar
   and sinvar_impl=sinvar
   and receiver_violation=SINVAR_SecGwExt.receiver_violation
-  and offending_flows_impl=SecurityGatewayExtended_offending_list
+  and offending_flows_impl=PolEnforcePointExtended_offending_list
   and node_props_impl=NetModel_node_props
-  and eval_impl=SecurityGateway_eval
+  and eval_impl=PolEnforcePoint_eval
  apply(unfold TopoS_List_Impl_def)
  apply(rule conjI)
-  apply(simp add: TopoS_SecurityGatewayExtended list_graph_to_graph_def)
+  apply(simp add: TopoS_PolEnforcePointExtended list_graph_to_graph_def)
  apply(rule conjI)
-  apply(simp add: list_graph_to_graph_def SecurityGatewayExtended_offending_set SecurityGatewayExtended_offending_set_def SecurityGatewayExtended_offending_list_def)
+  apply(simp add: list_graph_to_graph_def PolEnforcePointExtended_offending_set PolEnforcePointExtended_offending_set_def PolEnforcePointExtended_offending_list_def)
  apply(rule conjI)
   apply(simp only: NetModel_node_props_def)
-  apply(metis SecurityGatewayExtended.node_props.simps SecurityGatewayExtended.node_props_eq_node_props_formaldef)
- apply(simp only: SecurityGateway_eval_def)
- apply(simp add: TopoS_eval_impl_proofrule[OF TopoS_SecurityGatewayExtended])
+  apply(metis PolEnforcePointExtended.node_props.simps PolEnforcePointExtended.node_props_eq_node_props_formaldef)
+ apply(simp only: PolEnforcePoint_eval_def)
+ apply(simp add: TopoS_eval_impl_proofrule[OF TopoS_PolEnforcePointExtended])
  apply(simp_all add: list_graph_to_graph_def)
 done
 
 
-subsubsection {* SecurityGateway packing *}
-  definition SINVAR_LIB_SecurityGatewayExtended :: "('v::vertex, secgw_member) TopoS_packed" where
-    "SINVAR_LIB_SecurityGatewayExtended \<equiv> 
-    \<lparr> nm_name = ''SecurityGatewayExtended'', 
+subsubsection {* PolEnforcePoint packing *}
+  definition SINVAR_LIB_PolEnforcePointExtended :: "('v::vertex, secgw_member) TopoS_packed" where
+    "SINVAR_LIB_PolEnforcePointExtended \<equiv> 
+    \<lparr> nm_name = ''PolEnforcePointExtended'', 
       nm_receiver_violation = SINVAR_SecGwExt.receiver_violation,
       nm_default = SINVAR_SecGwExt.default_node_properties, 
       nm_sinvar = sinvar,
-      nm_offending_flows = SecurityGatewayExtended_offending_list, 
+      nm_offending_flows = PolEnforcePointExtended_offending_list, 
       nm_node_props = NetModel_node_props,
-      nm_eval = SecurityGateway_eval
+      nm_eval = PolEnforcePoint_eval
       \<rparr>"
-  interpretation SINVAR_LIB_SecurityGatewayExtended_interpretation: TopoS_modelLibrary SINVAR_LIB_SecurityGatewayExtended 
+  interpretation SINVAR_LIB_PolEnforcePointExtended_interpretation: TopoS_modelLibrary SINVAR_LIB_PolEnforcePointExtended 
       SINVAR_SecGwExt.sinvar
-    apply(unfold TopoS_modelLibrary_def SINVAR_LIB_SecurityGatewayExtended_def)
+    apply(unfold TopoS_modelLibrary_def SINVAR_LIB_PolEnforcePointExtended_def)
     apply(rule conjI)
      apply(simp)
     apply(simp)
@@ -77,7 +77,7 @@ text {* Examples*}
   definition example_conf_secgw where
   "example_conf_secgw \<equiv> ((\<lambda>e. SINVAR_SecGwExt.default_node_properties)
     (1 := DomainMember, 2:= DomainMember, 3:= AccessibleMember,
-     8:= SecurityGateway, 9:= SecurityGatewayIN))" 
+     8:= PolEnforcePoint, 9:= PolEnforcePointIN))" 
   
   export_code sinvar in SML
   definition "test = sinvar \<lparr> nodesL=[1::nat], edgesL=[] \<rparr> (\<lambda>_. SINVAR_SecGwExt.default_node_properties)"
@@ -85,14 +85,14 @@ text {* Examples*}
   value(**) "sinvar \<lparr> nodesL=[1::nat], edgesL=[] \<rparr> (\<lambda>_. SINVAR_SecGwExt.default_node_properties)"
 
   value(**) "sinvar example_net_secgw example_conf_secgw"
-  value(**) "SecurityGateway_offending_list example_net_secgw example_conf_secgw"
+  value(**) "PolEnforcePoint_offending_list example_net_secgw example_conf_secgw"
 
 
   definition example_net_secgw_invalid where
   "example_net_secgw_invalid \<equiv> example_net_secgw\<lparr>edgesL := (3,1)#(11,1)#(11,8)#(1,2)#(edgesL example_net_secgw)\<rparr>"
 
   value(**) "sinvar example_net_secgw_invalid example_conf_secgw"
-  value(**) "SecurityGateway_offending_list example_net_secgw_invalid example_conf_secgw"
+  value(**) "PolEnforcePoint_offending_list example_net_secgw_invalid example_conf_secgw"
 
 
 hide_const (open) NetModel_node_props
