thys/Network_Security_Policy_Verification/SINVAR_Examples.thy
@@ -311,13 +311,13 @@ end
 
 context begin
   private definition "secgwext_host_attributes \<equiv> [
-                             ''hypervisor'' \<mapsto> SecurityGateway,
+                             ''hypervisor'' \<mapsto> PolEnforcePoint,
                              ''securevm1'' \<mapsto> DomainMember,
                              ''securevm2'' \<mapsto> DomainMember,
                              ''publicvm1'' \<mapsto> AccessibleMember,
                              ''publicvm2'' \<mapsto> AccessibleMember
                              ]"
-  private definition "SecGwExt_m \<equiv> new_configured_list_SecurityInvariant SINVAR_LIB_SecurityGatewayExtended \<lparr> 
+  private definition "SecGwExt_m \<equiv> new_configured_list_SecurityInvariant SINVAR_LIB_PolEnforcePointExtended \<lparr> 
           node_properties = secgwext_host_attributes
           \<rparr> ''secure hypervisor mediates accesses between secure VMs''"
   private definition "secgwext_hosts \<equiv> [''hypervisor'', ''securevm1'', ''securevm2'',
@@ -335,14 +335,14 @@ context begin
 
   ML_val{*
   visualize_graph_header @{context} @{term "[SecGwExt_m, new_configured_list_SecurityInvariant SINVAR_LIB_BLPtrusted \<lparr> 
-        node_properties = [''hypervisor'' \<mapsto> \<lparr> privacy_level = 0, trusted = True \<rparr>,
-                           ''securevm1'' \<mapsto> \<lparr> privacy_level = 1, trusted = False \<rparr>,
-                           ''securevm2'' \<mapsto> \<lparr> privacy_level = 1, trusted = False \<rparr>
+        node_properties = [''hypervisor'' \<mapsto> \<lparr> security_level = 0, trusted = True \<rparr>,
+                           ''securevm1'' \<mapsto> \<lparr> security_level = 1, trusted = False \<rparr>,
+                           ''securevm2'' \<mapsto> \<lparr> security_level = 1, trusted = False \<rparr>
                            ] \<rparr> ''secure vms are confidential'']"}
     @{term "make_policy [SecGwExt_m, new_configured_list_SecurityInvariant SINVAR_LIB_BLPtrusted \<lparr> 
-        node_properties = [''hypervisor'' \<mapsto> \<lparr> privacy_level = 0, trusted = True \<rparr>,
-                           ''securevm1'' \<mapsto> \<lparr> privacy_level = 1, trusted = False \<rparr>,
-                           ''securevm2'' \<mapsto> \<lparr> privacy_level = 1, trusted = False \<rparr>
+        node_properties = [''hypervisor'' \<mapsto> \<lparr> security_level = 0, trusted = True \<rparr>,
+                           ''securevm1'' \<mapsto> \<lparr> security_level = 1, trusted = False \<rparr>,
+                           ''securevm2'' \<mapsto> \<lparr> security_level = 1, trusted = False \<rparr>
                            ] \<rparr> ''secure vms are confidential''] secgwext_hosts"}
     @{term "secgwext_host_attributes"};
   *}
